src/Examples/MailServer/MailTriples.v
@@ -84,8 +84,6 @@ Section refinement_triples.
      | _, _ => Count_Typed_Heap.mapsto (hG := go_heap_inG) p O (fst v) (snd v)
      end ∗ ⌜ p ≠ gmodel.(@nullptr) _⌝)%I (Data.allocs σ.(heap)).
 
-  Definition HeapInv_crash (σ: Mail.State) : iProp Σ := True%I.
-
   Definition InboxLockInv (γ: gname) (n: nat) :=
     (∃ S1 S2, ghost_mapsto_auth γ (A := discreteC contents) S1
       ∗ ghost_mapsto (A := discreteC contents) γ O S2)%I.
@@ -198,18 +196,9 @@ Section refinement_triples.
         ⌜ σ.(open) = true ⌝
       end)%I.
 
-  Definition InitInv_crash (Γ: gmap uint64 gname) γ σ :=
-    (ghost_mapsto_auth γ Uninit
-        ∗ ghost_mapsto γ O Uninit
-        ∗ ([∗ map] uid↦lm ∈ σ.(messages), ∃ γuid, ⌜ Γ !! uid = Some γuid ⌝ ∗ InboxLockInv γuid O))%I.
-
   Definition MsgsInv (Γ : gmap uint64 gname) (γ: gname) (σ: Mail.State) : iProp Σ :=
     (∃ ls, GlobalInv ls σ.(open) ∗ RootDirInv σ ∗ InitInv Γ γ σ
                      ∗ ([∗ map] uid↦lm ∈ σ.(messages), MsgInv Γ ls uid lm σ.(open)))%I.
-
-  Definition MsgsInv_crash (Γ : gmap uint64 gname) (γ: gname) (σ: Mail.State) : iProp Σ :=
-    (∃ ls, GlobalInv ls false ∗ RootDirInv σ ∗ InitInv_crash Γ γ σ
-                     ∗ ([∗ map] uid↦lm ∈ σ.(messages), MsgInv Γ ls uid lm false))%I.
 
   Lemma MsgInv_pers_split Γ ls uid lm :
     MsgInv Γ ls uid lm true -∗
@@ -243,19 +232,6 @@ Section refinement_triples.
     iFrame.
   Qed.
 
-  Lemma MsgsInv_crash_set_false Γ γ σ :
-    MsgsInv_crash Γ γ σ -∗ MsgsInv Γ γ (RecordSet.set open (λ _, false) σ).
-  Proof.
-    iIntros "H". iDestruct "H" as (ls) "(Hglobal&Hrootdir&Hinit&Hmsgs)".
-    iExists ls. iFrame.
-    rewrite /InitInv_crash/InitInv.
-    iExists Uninit. iDestruct "Hinit" as "($&$&$)". eauto.
-  Qed.
-
-  Global Instance MsgsInv_crash_timeless  Γ γ σ:
-    Timeless (MsgsInv_crash Γ γ σ).
-  Proof. apply _. Qed.
-
   Global Instance tmp_gen_mapsto `{gooseG Σ} : GenericMapsTo _ _
     := {| generic_mapsto := λ l q v, Count_GHeap.mapsto (hG := hGTmp) l q v|}%I.
 
@@ -263,11 +239,6 @@ Section refinement_triples.
     (∃ tmps_map, SpoolDir ↦ dom (gset string) tmps_map
                           ∗ SpoolDir ↦ Unlocked
                           ∗ gen_heap_ctx tmps_map
-                          ∗ [∗ map] name↦inode ∈ tmps_map,
-                                      path.mk SpoolDir name ↦ inode
-                                      (* ∗ name ↦{1} inode *) )%I.
-  Definition TmpInv_crash : iProp Σ :=
-    (∃ tmps_map, SpoolDir ↦{1} dom (gset string) tmps_map
                           ∗ [∗ map] name↦inode ∈ tmps_map,
                                       path.mk SpoolDir name ↦ inode
                                       (* ∗ name ↦{1} inode *) )%I.
@@ -290,18 +261,6 @@ Section refinement_triples.
 
   Definition ExecInner :=
     (∃ Γ γ σ, ⌜ σ.(open) = false ⌝ ∗ source_state σ ∗ MsgsInv Γ γ σ ∗ HeapInv σ ∗ TmpInv)%I.
-
-  Definition CrashInv :=
-    (∃ Γ γ, source_ctx
-              ∗ inv execN (∃ σ, source_state σ ∗ MsgsInv_crash Γ γ σ
-              ∗ HeapInv_crash σ ∗ TmpInv_crash))%I.
-
-  Definition CrashStarter :=
-    (∃ tmps : gset string, SpoolDir ↦{-1} tmps ∗ SpoolDir ↦ Unlocked)%I.
-
-  Definition CrashInner :=
-    ((∃ Γ γ σ, source_state σ ∗ MsgsInv_crash Γ γ σ
-               ∗ HeapInv_crash σ ∗ TmpInv_crash) ∗ CrashStarter)%I.
 
   Lemma GlobalInv_unify lsptr ls ls':
     global ↦{-1} Some lsptr -∗ lsptr ↦{-1} (ls, ls) -∗ GlobalInv ls' true -∗ ⌜ ls = ls' ⌝.
